dist/experiment.h
@@ -18,6 +18,10 @@ void Experiment_Steel_Test_Extract_test3_LV_(uint32_t *r0, uint32_t *r1);
 
 uint32_t Experiment_Steel_Test_Extract_test_ghost(uint32_t *r);
 
+void Experiment_Steel_Test_Extract_test_slrewrite(uint32_t *r0, uint32_t *r1, uint32_t *r2);
+
+void Experiment_Steel_Test_Extract_test_with_invariant_g(uint32_t *r1);
+
 
 #define __experiment_H_DEFINED
 #endif
