experiment/Experiment.Steel.GCombinators.fst
@@ -1,53 +1,32 @@
 module Experiment.Steel.GCombinators
 
-module U    = Learn.Util
-module L    = FStar.List.Pure
-module M    = Experiment.Steel.Repr.M
-module MC   = Experiment.Steel.Combinators
-module LV   = Experiment.Steel.Repr.LV
-module SF   = Experiment.Steel.Repr.SF
-module SH   = Experiment.Steel.Steel
-module Ll   = Learn.List
-module Fl   = Learn.FList
-module Veq  = Experiment.Steel.VEquiv
-module Mem  = Steel.Memory
-module Perm = Learn.Permutation
+module U      = Learn.Util
+module L      = FStar.List.Pure
+module M      = Experiment.Steel.Repr.M
+module MC     = Experiment.Steel.Combinators
+module LV     = Experiment.Steel.Repr.LV
+module SF     = Experiment.Steel.Repr.SF
+module SH     = Experiment.Steel.Steel
+module Ll     = Learn.List
+module Dl     = Learn.DList
+module Fl     = Learn.FList
+module SA     = Steel.Effect.Atomic
+module Veq    = Experiment.Steel.VEquiv
+module Msk    = Learn.List.Mask
+module Mem    = Steel.Memory
+module Perm   = Learn.Permutation
+module LV2M   = Experiment.Steel.Repr.LV_to_M
+module LV2SF  = Experiment.Steel.Repr.LV_to_SF
+module TLogic = Learn.Tactics.Logic
 
 open Steel.Effect
 open Steel.Effect.Atomic
 open Experiment.Steel.VPropList
 open Experiment.Steel.Interface
 open FStar.Tactics
-open Experiment.Steel.Tac
+open Experiment.Steel.GCombinators.Lib
 
 #set-options "--fuel 1 --ifuel 1"
-
-#push-options "--fuel 0 --ifuel 0"
-//TODO? inline s
-inline_for_extraction
-let make_combinator_steel_ghost
-      (#a : Type u#a) (opened : Mem.inames) (s : M.spec_r a) (f : M.spc_steel_t (SH.KGhost opened) s)
-      (#pre : M.pre_t) (pre_eq : Veq.vequiv pre (M.spc_pre1 s))
-      (#post : M.post_t a) (post_eq : ((x : a) -> Veq.vequiv (M.spc_post1 s x) (post x)))
-  : M.repr_steel_t (SH.KGhost opened) a pre post (M.gen_req s pre_eq post_eq) (M.gen_ens s pre_eq post_eq)
-  =
-    SH.ghost_f #opened (fun () ->
-      pre_eq.veq_g _;
-      (**) steel_elim_vprop_of_list_append_f s.spc_pre s.spc_ro;
-      (**) let sl0'  = gget_f s.spc_pre in
-      (**) let sl_ro = gget_f s.spc_ro in     
-      (**) assert (s.spc_req sl0' sl_ro);
-      let (x : a) = SH.ghost_u f () in
-      (**) let sl1'   = gget_f (s.spc_post x) in
-      (**) let sl_ro' = gget_f s.spc_ro       in
-      (**) assert (sl_ro' == sl_ro);
-      (**) assert (s.spc_ens sl0' x sl1' sl_ro);
-      (**) steel_intro_vprop_of_list_append_f (s.spc_post x) s.spc_ro;
-      (post_eq x).veq_g _;
-      x
-    )
-#pop-options
-    
 
 (**** slrewrite *)
 
@@ -117,35 +96,374 @@ let build_slrewrite (fr : flags_record) : Tac unit
     trefl ()
 
 [@@ __repr_M__]
-let slrewrite_M_tree (#t : Type u#t) (x0 x1 : t)
-  : M.prog_tree (U.unit' u#a)
-  = M.Tgen (U.unit' u#a) build_slrewrite (slrewrite_gen_c #t x0 x1)
-
-[@@ __repr_M__]
 inline_for_extraction
 let slrewrite (#t : Type u#t) (#opened : Mem.inames) (x0 x1 : t)
   : M.repr (SH.KGhost opened) (U.unit' u#a)
-  = {
-    repr_tree  = slrewrite_M_tree x0 x1;
-    repr_steel = (fun pre post c ->
-                    let M.TCgen s sh _ pre_eq _ post_eq = c in
-                    let SlRewrite v0 v1 frame veq = U.cast (slrewrite_gen_c #t x0 x1 s) sh in
-                    make_combinator_steel_ghost opened s
-                      (slrewrite_steel opened x0 x1 v0 v1 frame veq)
-                      pre_eq post_eq)
-  }
+  =
+    make_combinator (U.unit' u#a) (SH.KGhost opened) build_slrewrite (slrewrite_gen_c #t x0 x1)
+      (fun _ (SlRewrite v0 v1 frame veq) -> slrewrite_steel opened x0 x1 v0 v1 frame veq)
 
 
-module F   = Experiment.Steel.Notations
-module U32 = FStar.UInt32
-open Steel.Reference
+(**** with_invariant_g *)
 
-let test_slrewrite (r0 r1 r2 : ref U32.t)
-  : F.steel unit
-      (vptr r0 `star` vptr r1) (fun _ -> vptr r2 `star` vptr r1)
-      (requires fun _ -> r0 == r2)
-      (ensures  fun h0 _ h1 -> sel r0 h0 == sel r2 h1 /\ sel r1 h0 == sel r1 h1)
-  = F.(to_steel (
-      MC.ghost_to_steel_ct (slrewrite r0 r2) (fun _ -> U.Unit');;
-      return ()
-    ) ())
+#push-options "--ifuel 0 --fuel 0"
+
+// FIXME: raises warning 271 about theory symbols in pattern on the exists of ref_post
+#push-options "--fuel 1 --warn_error -271"
+
+/// A version of [with_invariant_g] with selectors.
+inline_for_extraction
+let with_invariant_g_sl
+      (#a : Type)
+      (pre : pre_t) (post : post_t a)
+      (#opened : Mem.inames)
+      (#p : vprop)
+      (i : inv p { not (mem_inv opened i) })
+      (req : t_of p -> t_of pre -> Type0) (ens : t_of p -> t_of pre -> (x : a) -> t_of p -> t_of (post x) -> Type0)
+      (f : unit -> SteelGhost a (add_inv opened i)
+                    (p `star` pre) (fun x -> p `star` (post x))
+                    (requires fun h0      -> req (h0 p) (h0 pre))
+                    (ensures  fun h0 x h1 -> ens (h0 p) (h0 pre) x (h1 p) (h1 (post x))))
+  : SteelGhost a opened pre post
+      (requires fun h0      -> forall (sl_p0 : t_of p) . req sl_p0 (h0 pre))
+      (ensures  fun h0 x h1 -> exists (sl_p0 sl_p1 : t_of p) . ens sl_p0 (h0 pre) x sl_p1 (h1 (post x)))
+  =
+    let sl_pre = gget pre                                           in
+    let ref_pre  (sl_pre' : t_of pre) : prop
+      = sl_pre' == Ghost.reveal sl_pre                              in
+    let ref_post (x : a) (sl_post : t_of (post x)) : prop
+      = exists (sl_p0 sl_p1 : t_of p) . ens sl_p0 sl_pre x sl_p1 sl_post in
+    intro_vrefine pre ref_pre;
+    let x = SA.with_invariant_g
+      #a #(vrefine pre ref_pre) #(fun x -> vrefine (post x) (ref_post x))
+      #opened #p i
+      (fun () -> begin
+        let sl_p0   = gget p        in
+        elim_vrefine pre ref_pre;
+        let sl_pre' = gget pre      in
+        U.assert_by (sl_pre' == sl_pre) (fun () ->
+          assert (Ghost.reveal sl_pre' == Ghost.reveal sl_pre);
+          Ghost.hide_reveal sl_pre;
+          Ghost.hide_reveal sl_pre');
+        eliminate forall (sl_p0 : t_of p) . req sl_p0 sl_pre
+          with sl_p0;
+        let x = f () in
+        let sl_p1   = gget p        in
+        let sl_post = gget (post x) in
+        introduce exists (sl_p0 sl_p1 : t_of p) . ens sl_p0 sl_pre x sl_p1 sl_post
+          with sl_p0 sl_p1 and ();
+        intro_vrefine (post x) (ref_post x);
+        x
+      end <: SteelGhostT a (add_inv opened i)
+               (p `star` vrefine pre ref_pre) (fun x -> p `star` vrefine (post x) (ref_post x)))
+    in
+    elim_vrefine (post x) (ref_post x);
+    x
+
+let change_equiv_slprop
+      (#opened : Mem.inames)
+      (p q : vprop)
+      (l : unit -> Lemma (p `equiv` q))
+  : SteelGhostT unit opened p (fun _ -> q)
+  =
+    rewrite_slprop p q (fun m -> l (); equiv_can_be_split p q; can_be_split_interp p q m)
+
+/// A variant for changing [p] into an equivalent [vprop] (in practice a [vprop_of_list _]).
+/// TODO? selector bijection instead : v <-> vprop_of_list (flatten_vprop _)
+inline_for_extraction
+let with_invariant_g_sl_list
+      (#a : Type)
+      (pre : pre_t) (post : post_t a)
+      (#opened : Mem.inames)
+      (#p : vprop)
+      (i : inv p { not (mem_inv opened i) })
+      (p' : vprop) (_ : squash (p `equiv` p'))//FIXME? Steel tactics fail if we put it as a refinement on p'
+      (req : t_of p' -> t_of pre -> Type0) (ens : t_of p' -> t_of pre -> (x : a) -> t_of p' -> t_of (post x) -> Type0)
+      (f : unit -> SteelGhost a (add_inv opened i)
+                    (p' `star` pre) (fun x -> p' `star` (post x))
+                    (requires fun h0      -> req (h0 p') (h0 pre))
+                    (ensures  fun h0 x h1 -> ens (h0 p') (h0 pre) x (h1 p') (h1 (post x))))
+  : SteelGhost a opened pre post
+      (requires fun h0      -> forall (sl_p0 : t_of p') . req sl_p0 (h0 pre))
+      (ensures  fun h0 x h1 -> exists (sl_p0 sl_p1 : t_of p') . ens sl_p0 (h0 pre) x sl_p1 (h1 (post x)))
+  =
+    let sl_pre = gget pre                                           in
+    let ref_pre  (sl_pre' : t_of pre) : prop
+      = sl_pre' == Ghost.reveal sl_pre                              in
+    let ref_post (x : a) (sl_post : t_of (post x)) : prop
+      = exists (sl_p0 sl_p1 : t_of p') . ens sl_p0 sl_pre x sl_p1 sl_post in
+    intro_vrefine pre ref_pre;
+    let x = SA.with_invariant_g
+      #a #(vrefine pre ref_pre) #(fun x -> vrefine (post x) (ref_post x))
+      #opened #p i
+      (fun () -> begin
+        change_equiv_slprop p p' (fun () -> ());
+        slassert (p' `star` vrefine pre ref_pre);
+        let sl_p0   = gget p'       in
+        elim_vrefine pre ref_pre;
+        let sl_pre' = gget pre      in
+        (U.assert_by (sl_pre' == sl_pre) (fun () ->
+          assert (Ghost.reveal sl_pre' == Ghost.reveal sl_pre);
+          Ghost.hide_reveal sl_pre;
+          Ghost.hide_reveal sl_pre');
+        eliminate forall (sl_p0 : t_of p') . req sl_p0 sl_pre
+          with sl_p0;
+        ());
+        let x = f () in
+        let sl_p1   = gget p'       in
+        let sl_post = gget (post x) in
+        (introduce exists (sl_p0 sl_p1 : t_of p') . ens sl_p0 sl_pre x sl_p1 sl_post
+          with sl_p0 sl_p1 and ();
+        ());
+        intro_vrefine (post x) (ref_post x);
+        change_equiv_slprop p' p (fun () -> equiv_sym p p');
+        x
+      end <: SteelGhostT a (add_inv opened i)
+               (p `star` vrefine pre ref_pre) (fun x -> p `star` vrefine (post x) (ref_post x)))
+    in
+    elim_vrefine (post x) (ref_post x);
+    x
+
+#pop-options
+
+
+let with_invariant_inner_spec_r
+     (#a : Type u#a) (p : vprop_list)
+     (pre : M.pre_t) (post : M.post_t a) (ro : vprop_list)
+     (req : sl_f L.(p @ pre) -> sl_f ro -> Type0)
+     (ens : sl_f L.(p @ pre) -> (x : a) -> sl_f L.(p @ post x) -> sl_f ro -> Type0)
+  : M.spec_r a
+  = M.Mkspec_r L.(p @ pre) L.(fun x -> p @ post x) ro req ens
+
+[@@ __cond_solver__]
+let with_invariant_spec_r
+     (#a : Type u#a) (p : vprop_list)
+     (pre : M.pre_t) (post : M.post_t a) (ro : vprop_list)
+     (req : sl_f L.(p @ pre) -> sl_f ro -> Type0)
+     (ens : sl_f L.(p @ pre) -> (x : a) -> sl_f L.(p @ post x) -> sl_f ro -> Type0)
+  : M.spec_r a
+  =
+    M.Mkspec_r
+       pre post ro
+       (fun sl0 sl_ro ->
+          forall (sl_p0 : sl_f p) . req (append_vars sl_p0 sl0) sl_ro)
+       (fun sl0 x sl1 sl_ro ->
+         exists (sl_p0 sl_p1 : sl_f p) . ens (append_vars sl_p0 sl0) x (append_vars sl_p1 sl1) sl_ro)
+
+
+(* Does not work (universes)
+noeq
+type with_invariant_gen_c
+     (#a : Type u#a) (p : vprop) (f : M.prog_tree a)
+  : M.spec_r a -> Type u#(max a 2) =
+  | WithInvariant :
+      (p' : vprop_to_list p) ->
+      (env : vprop_list) -> (csm : LV.csm_t env) -> (prd : LV.prd_t a) ->
+      (cf : LV.lin_cond L.(p' @ env) f (LV.bind_g_csm' p' csm) (fun x -> L.(p' @ prd x))) ->
+      with_invariant_gen_c p f (with_invariant_spec_r_lc p' cf)
+*)
+
+/// [f] is mentioned only to be recovered by [__build_with_invariant]. Since it is a parameter, it does not
+/// affect the universe of the datatype.
+noeq
+type with_invariant_gen_c (a : Type u#a) (ek : SH.effect_kind) (f : M.repr ek a) (p : vprop)
+  : M.spec_r a -> Type u#(max a 2) =
+  | WithInvariant :
+      (p' : vprop_list) -> (tp : vprop_to_list p p') ->
+      (pre : M.pre_t) -> (post : M.post_t a) -> (ro : vprop_list) ->
+      (req : (sl_f L.(p' @ pre) -> sl_f ro -> Type0)) ->
+      (ens : (sl_f L.(p' @ pre) -> (x : a) -> sl_f L.(p' @ post x) -> sl_f ro -> Type0)) ->
+      (inner : M.spc_steel_t ek (with_invariant_inner_spec_r p' pre post ro req ens)) ->
+      with_invariant_gen_c a ek f p (with_invariant_spec_r p' pre post ro req ens)
+
+
+#push-options "--fuel 1 --z3rlimit 20"
+inline_for_extraction
+let with_invariant_g_steel
+      (a : Type u#a) (opened : Mem.inames)
+      (#p : vprop) (i : inv p{not (mem_inv opened i)})
+      (p' : vprop_list) (tp : vprop_to_list p p')
+      (pre : M.pre_t) (post : M.post_t a) (ro : vprop_list)
+      (req : sl_f L.(p' @ pre) -> sl_f ro -> Type0)
+      (ens : sl_f L.(p' @ pre) -> (x : a) -> sl_f L.(p' @ post x) -> sl_f ro -> Type0)
+      (inner : M.spc_steel_t (SH.KGhost (add_inv opened i)) (with_invariant_inner_spec_r p' pre post ro req ens))
+  : M.spc_steel_t (SH.KGhost opened) (with_invariant_spec_r p' pre post ro req ens)
+  = SH.ghost_f #opened (fun () ->
+    (**) (vprop_to_list_equiv tp; ());
+    with_invariant_g_sl_list
+      (vprop_of_list pre `star` vprop_of_list ro)
+      (fun x -> vprop_of_list (post x) `star` vprop_of_list ro)
+      i (vprop_of_list p') ()
+      (fun sl_p0 sl0 ->
+        req (append_vars (vpl_sels_f p' sl_p0) (vpl_sels_f pre sl0._1)) (vpl_sels_f ro sl0._2))
+      (fun sl_p0 sl0 x sl_p1 sl1 ->
+        ens (append_vars (vpl_sels_f p' sl_p0) (vpl_sels_f pre sl0._1)) x
+            (append_vars (vpl_sels_f p' sl_p1) (vpl_sels_f (post x) sl1._1)) (vpl_sels_f ro sl0._2) /\
+        vpl_sels_f ro sl1._2 == vpl_sels_f ro sl0._2)
+    begin fun () ->
+      (**) steel_intro_vprop_of_list_append_f p' pre;
+      let x = SH.ghost_u inner () in
+      (**) steel_elim_vprop_of_list_append_f p' (post x);
+      x
+    end
+  )
+#pop-options
+
+[@@ __cond_solver__]
+let with_invariant_spec_r_lc
+     (#a : Type u#a) (p : vprop_list) (#f : M.prog_tree a)
+     (#env : vprop_list) (csm : LV.csm_t env) (#prd : LV.prd_t a)
+     (cf : LV.lin_cond L.(p @ env) f (LV.bind_g_csm' p csm) L.(fun x -> p @ prd x))
+  : M.spec_r a
+  =
+    (**) LV.filter_csm_bind_g_csm' p csm;
+    (**) LV.filter_bind_g_csm'     p csm;
+    with_invariant_spec_r p Msk.(filter_mask csm env) prd Msk.(filter_mask (mask_not csm) env)
+                          (lc_req cf) (lc_ens cf)
+
+// TODO? use __LV2SF__ operations instead of append_vars & split_vars
+[@@ __LV2SF__]
+let with_invariant_sf'
+      (#a : Type u#a) (p : vprop_list) (#f : M.prog_tree a)
+      (#env : vprop_list) (csm : LV.csm_t env) (#prd : LV.prd_t a)
+      (cf : LV.lin_cond L.(p @ env) f (LV.bind_g_csm' p csm) L.(fun x -> p @ prd x))
+      (sl0 : sl_f Msk.(filter_mask csm env)) (sl_ro : sl_f Msk.(filter_mask (mask_not csm) env))
+  : SF.prog_tree a (M.post_sl_t prd)
+  =
+    (**) LV.filter_csm_bind_g_csm' p csm;
+    (**) LV.filter_bind_g_csm'     p csm;
+  SF.(
+    Tbind _ _ (fun _ -> vprop_list_sels_t p) _
+      (Tspec U.unit' (fun _ -> vprop_list_sels_t p) True (fun _ _ -> True)) (fun _ sl_p0 ->
+   (Tbind _ _ L.(fun x -> vprop_list_sels_t (p @ prd x)) _
+      (lc_sf cf (append_vars sl_p0 sl0) sl_ro) (fun x sl1' ->
+      (Tret a x (M.post_sl_t prd) (Fl.dlist_of_f (split_vars p (prd x) sl1')._2))
+  ))))
+
+
+let force_tree_req #a (#post : SF.post_t a) (t : SF.prog_tree a post)
+  : squash (SF.tree_req t <==> SF.tree_req t)
+  = ()
+
+let force_tree_ens #a (#post : SF.post_t a) (t : SF.prog_tree a post) x sl1
+  : squash (SF.tree_ens t x sl1 <==> SF.tree_ens t x sl1)
+  = ()
+
+let __normal_with_invariant_sf : list norm_step = [
+  delta_only [`%with_invariant_sf'; `%with_invariant_spec_r_lc; `%with_invariant_spec_r;
+              `%M.Mkspec_r?.spc_req; `%M.Mkspec_r?.spc_ens; `%M.Mkspec_r?.spc_post;
+              `%SF.tree_req; `%SF.tree_ens;
+              `%SF.post_v; `%sl_f; `%lc_spec_r; `%lc_post; `%M.post_sl_t];
+  iota; zeta; simplify
+]
+
+[@@ __LV2SF__]
+let with_invariant_sf
+      (#a : Type u#a) (p : vprop_list) (#f : M.prog_tree a)
+      (#env : vprop_list) (csm : LV.csm_t env) (#prd : LV.prd_t a)
+      (cf : LV.lin_cond L.(p @ env) f (LV.bind_g_csm' p csm) L.(fun x -> p @ prd x))
+  : LV.gen_sf (with_invariant_spec_r_lc p csm cf)
+  =
+    fun sl0 sl_ro ->
+      (**) LV.filter_csm_bind_g_csm' p csm;
+      (**) LV.filter_bind_g_csm'     p csm;
+      let t = with_invariant_sf' p csm cf sl0 sl_ro in
+      let s = with_invariant_spec_r_lc p csm cf     in
+      let rew_req sl0'
+        : Lemma (SF.tree_req (lc_sf cf sl0' sl_ro) <==> lc_req cf sl0' sl_ro)
+        = ()
+      in
+      assert (SF.tree_req t <==> s.spc_req sl0 sl_ro)
+        by (norm __normal_with_invariant_sf;
+            apply (`TLogic.rew_iff_left); apply (`force_tree_req);
+            norm __normal_with_invariant_sf;
+            apply (`TLogic.rew_iff_left );
+              TLogic.rew_iff (fun r -> fail "");
+            apply (`TLogic.rew_iff_right);
+              TLogic.rew_iff (fun r -> apply (`rew_lc_sf_req));
+            norm __normal_with_invariant_sf;
+            smt ());
+
+      introduce forall (x : a) (sl1 : sl_f (s.spc_post x)) .
+                SF.tree_ens t x sl1 <==> s.spc_ens sl0 x sl1 sl_ro
+      with begin
+        U.assert_by_tac (fun () ->
+            norm __normal_with_invariant_sf;
+            apply (`TLogic.rew_iff_left); apply (`force_tree_ens);
+            norm __normal_with_invariant_sf;
+            apply (`TLogic.rew_iff_left);
+              TLogic.rew_iff (fun r -> fail "");
+              norm [];
+            apply (`TLogic.exists_morph_iff); let sl_p0 = intro () in
+            apply (`TLogic.rew_iff_right);
+              TLogic.rew_iff (fun r -> apply (`rew_lc_sf_ens));
+            apply (`TLogic.rew_iff_left);
+              TLogic.rew_iff (fun r -> apply (`rew_exists_sl_f_app); r ());
+              norm [];
+            l_to_r [`append_split_vars]; norm [delta_only [`%Mktuple2?._2]; iota];
+            norm __normal_with_invariant_sf;
+            smt ()
+        )
+      end;
+
+      t
+
+
+[@@ __cond_solver__]
+let __build_with_invariant
+      (env : vprop_list)
+      (#a : Type u#a) (#ek : SH.effect_kind) (f : M.repr ek a) (#p : vprop) (#gen_tac : M.gen_tac_t)
+      (p' : vprop_list) (tp : vprop_to_list p p')
+      (csm : LV.csm_t env) (prd : LV.prd_t a)
+      (cf : (Msk.filter_mask_split_l (L.length p') (L.length env) p' env;
+             lin_cond_st L.(p' @ env) (let M.Mkrepr t _ = f in t)
+               (Msk.mask_split_l (L.length p') (L.length env)) (fun _ -> p')
+               csm prd))
+  : LV.lin_cond env (M.Tgen a gen_tac (with_invariant_gen_c a ek f p)) csm prd
+  =
+    let n_p'  = L.length p'                 in
+    let n_env = L.length env                in
+    let csm0  = Msk.mask_split_l n_p' n_env in
+    (**) LV.filter_csm_bind_g_csm' p' csm;
+    (**) LV.filter_bind_g_csm'     p' csm;
+    U.assert_by (Msk.mask_comp_or csm0 csm == LV.bind_g_csm' p' csm) (fun () ->
+      LV.bind_g_csm'_as_comp_or p' csm);
+    let pre = Msk.(filter_mask csm env)            in
+    let ro  = Msk.(filter_mask (mask_not csm) env) in
+    assert (lc_pre cf == L.(p' @ pre));
+    assert (lc_ro  cf == ro);
+    let s  = with_invariant_spec_r_lc p' csm cf    in
+    let sf = with_invariant_sf        p' csm cf    in
+    let pre_f : Perm.pequiv_list env (M.spc_pre1 s)
+      = Perm.perm_f_to_list (Msk.mask_pequiv_append csm env)  in
+    LV.gen_csm_pequiv_append env csm;
+    assert (LV.gen_csm pre_f == csm);
+    LV.LCgen env s
+      (WithInvariant p' tp pre prd ro (lc_req cf) (lc_ens cf) (lc_to_spc_steel_t f cf))
+      pre_f sf
+
+let build_with_invariant_g (fr : flags_record) : Tac unit
+  =
+    let ctx () = [Info_location "in with_invariant_g"] in
+    apply (`__build_with_invariant);
+    // tp
+    build_vprop_to_list fr ctx;
+    // cf
+    norm_lc ();
+    build_lin_cond_st fr ctx
+
+
+[@@ __repr_M__]
+inline_for_extraction
+let with_invariant_g
+      (#a : Type u#a) (#opened : Mem.inames)
+      (#p : vprop) (i : inv p{not (mem_inv opened i)})
+      (f : M.repr (SH.KGhost (add_inv opened i)) a)
+  : M.repr (SH.KGhost opened) a
+  =
+    make_combinator a (SH.KGhost opened)
+      build_with_invariant_g (with_invariant_gen_c a (SH.KGhost (add_inv opened i)) f p)
+      (fun _ (WithInvariant p' tp pre post ro req ens inner) ->
+         with_invariant_g_steel a opened i p' tp pre post ro req ens inner)
+
+#pop-options
