experiment/Experiment.Steel.GCombinators.Lib.fst
@@ -1,0 +1,540 @@
+module Experiment.Steel.GCombinators.Lib
+
+include Experiment.Steel.Tac
+include Experiment.Steel.Tac.LV
+
+module U     = Learn.Util
+module L     = FStar.List.Pure
+module M     = Experiment.Steel.Repr.M
+module Ll    = Learn.List
+module Fl    = Learn.FList
+module SH    = Experiment.Steel.Steel
+module LV    = Experiment.Steel.Repr.LV
+module SF    = Experiment.Steel.Repr.SF
+module SA    = Steel.Effect.Atomic
+module Veq   = Experiment.Steel.VEquiv
+module Mem   = Steel.Memory
+module Msk   = Learn.List.Mask
+module Perm  = Learn.Permutation
+module LV2M  = Experiment.Steel.Repr.LV_to_M
+module LV2SF = Experiment.Steel.Repr.LV_to_SF
+
+open Steel.Effect
+open Steel.Effect.Atomic
+open Experiment.Steel.VPropList
+open Experiment.Steel.Interface
+open FStar.Tactics
+
+#set-options "--fuel 1 --ifuel 1"
+
+
+(*** [make_combinator] *)
+
+/// [make_combinator] is used to build a new combinator. It handle the [pre_eq] and [post_eq] of [M.TCgen].
+
+#push-options "--fuel 0 --ifuel 0"
+inline_for_extraction
+let make_combinator_steel
+      (#a : Type u#a) (s : M.spec_r a) (f : M.spc_steel_t SH.KSteel s)
+      (#pre : M.pre_t) (pre_eq : Veq.vequiv pre (M.spc_pre1 s))
+      (#post : M.post_t a) (post_eq : ((x : a) -> Veq.vequiv (M.spc_post1 s x) (post x)))
+  : M.repr_steel_t SH.KSteel a pre post (M.gen_req s pre_eq post_eq) (M.gen_ens s pre_eq post_eq)
+  =
+    SH.steel_f (fun () ->
+      pre_eq.veq_g _;
+      (**) steel_elim_vprop_of_list_append_f s.spc_pre s.spc_ro;
+      (**) let sl0'  = gget_f s.spc_pre in
+      (**) let sl_ro = gget_f s.spc_ro in     
+      (**) assert (s.spc_req sl0' sl_ro);
+      let (x : a) = SH.steel_u f () in
+      (**) let sl1'   = gget_f (s.spc_post x) in
+      (**) let sl_ro' = gget_f s.spc_ro       in
+      (**) assert (sl_ro' == sl_ro);
+      (**) assert (s.spc_ens sl0' x sl1' sl_ro);
+      (**) steel_intro_vprop_of_list_append_f (s.spc_post x) s.spc_ro;
+      (post_eq x).veq_g _;
+      SA.return x
+    )
+
+inline_for_extraction
+let make_combinator_steel_atomic
+      (#a : Type u#a) (opened : Mem.inames) (s : M.spec_r a) (f : M.spc_steel_t (SH.KAtomic opened) s)
+      (#pre : M.pre_t) (pre_eq : Veq.vequiv pre (M.spc_pre1 s))
+      (#post : M.post_t a) (post_eq : ((x : a) -> Veq.vequiv (M.spc_post1 s x) (post x)))
+  : M.repr_steel_t (SH.KAtomic opened) a pre post (M.gen_req s pre_eq post_eq) (M.gen_ens s pre_eq post_eq)
+  =
+    SH.atomic_f #opened (fun () ->
+      pre_eq.veq_g _;
+      (**) steel_elim_vprop_of_list_append_f s.spc_pre s.spc_ro;
+      (**) let sl0'  = gget_f s.spc_pre in
+      (**) let sl_ro = gget_f s.spc_ro in     
+      (**) assert (s.spc_req sl0' sl_ro);
+      let (x : a) = SH.atomic_u f () in
+      (**) let sl1'   = gget_f (s.spc_post x) in
+      (**) let sl_ro' = gget_f s.spc_ro       in
+      (**) assert (sl_ro' == sl_ro);
+      (**) assert (s.spc_ens sl0' x sl1' sl_ro);
+      (**) steel_intro_vprop_of_list_append_f (s.spc_post x) s.spc_ro;
+      (post_eq x).veq_g _;
+      SA.return x
+    )
+
+inline_for_extraction
+let make_combinator_steel_ghost
+      (#a : Type u#a) (opened : Mem.inames) (s : M.spec_r a) (f : M.spc_steel_t (SH.KGhost opened) s)
+      (#pre : M.pre_t) (pre_eq : Veq.vequiv pre (M.spc_pre1 s))
+      (#post : M.post_t a) (post_eq : ((x : a) -> Veq.vequiv (M.spc_post1 s x) (post x)))
+  : M.repr_steel_t (SH.KGhost opened) a pre post (M.gen_req s pre_eq post_eq) (M.gen_ens s pre_eq post_eq)
+  =
+    SH.ghost_f #opened (fun () ->
+      pre_eq.veq_g _;
+      (**) steel_elim_vprop_of_list_append_f s.spc_pre s.spc_ro;
+      (**) let sl0'  = gget_f s.spc_pre in
+      (**) let sl_ro = gget_f s.spc_ro in     
+      (**) assert (s.spc_req sl0' sl_ro);
+      let (x : a) = SH.ghost_u f () in
+      (**) let sl1'   = gget_f (s.spc_post x) in
+      (**) let sl_ro' = gget_f s.spc_ro       in
+      (**) assert (sl_ro' == sl_ro);
+      (**) assert (s.spc_ens sl0' x sl1' sl_ro);
+      (**) steel_intro_vprop_of_list_append_f (s.spc_post x) s.spc_ro;
+      (post_eq x).veq_g _;
+      x
+    )
+#pop-options
+
+inline_for_extraction
+let make_combinator_steel_ek
+      (ek : SH.effect_kind) (#a : Type u#a) (s : M.spec_r a) (f : M.spc_steel_t ek s)
+      (#pre : M.pre_t) (pre_eq : Veq.vequiv pre (M.spc_pre1 s))
+      (#post : M.post_t a) (post_eq : ((x : a) -> Veq.vequiv (M.spc_post1 s x) (post x)))
+  : M.repr_steel_t ek a pre post (M.gen_req s pre_eq post_eq) (M.gen_ens s pre_eq post_eq)
+  = match ek with
+  | SH.KSteel         -> make_combinator_steel               s f pre_eq post_eq
+  | SH.KAtomic opened -> make_combinator_steel_atomic opened s f pre_eq post_eq
+  | SH.KGhost  opened -> make_combinator_steel_ghost  opened s f pre_eq post_eq
+
+[@@ __repr_M__]
+inline_for_extraction
+let make_combinator
+      (a : Type u#a) (ek : SH.effect_kind) (gen_tac : M.gen_tac_t) (gen_c : M.spec_r a -> Type u#(max a 2))
+      (f : (s : M.spec_r a) -> (sh : gen_c s) -> M.spc_steel_t ek s)
+  : M.repr ek a
+  = {
+    repr_tree  = M.Tgen a gen_tac gen_c;
+    repr_steel = (fun pre post c ->
+                    let M.TCgen s sh _ pre_eq _ post_eq = c in
+                    make_combinator_steel_ek ek s (f s sh) pre_eq post_eq)
+  }
+
+
+(*** [lc_spec_r] *)
+
+/// [lc_spec_r lc] is the specification (given as a [M.spec_r]) resulting from the [LV.lin_cond] [lc].
+/// [lc_sf] provides a corresponding [gen_sf] (that is a [SF.prog_tree] with an equivalent specification).
+/// [lc_to_spc_steel_t] gives a Steel implementation.
+
+[@@ __cond_solver__; __LV2SF__]
+let lc_pre
+      (#a : Type u#a) (#env : vprop_list) (#t : M.prog_tree a) (#csm : LV.csm_t env) (#prd : LV.prd_t a)
+      (lc : LV.lin_cond env t csm prd)
+  : M.pre_t
+  = Msk.(filter_mask csm env)
+
+[@@ __cond_solver__; __LV2SF__]
+let lc_post
+      (#a : Type u#a) (#env : vprop_list) (#t : M.prog_tree a) (#csm : LV.csm_t env) (#prd : LV.prd_t a)
+      (lc : LV.lin_cond env t csm prd)
+  : M.post_t a
+  = prd
+
+[@@ __cond_solver__; __LV2SF__]
+let lc_ro
+      (#a : Type u#a) (#env : vprop_list) (#t : M.prog_tree a) (#csm : LV.csm_t env) (#prd : LV.prd_t a)
+      (lc : LV.lin_cond env t csm prd)
+  : vprop_list
+  = Msk.(filter_mask (mask_not csm) env)
+
+let lc_req
+      (#a : Type u#a) (#env : vprop_list) (#t : M.prog_tree a) (#csm : LV.csm_t env) (#prd : LV.prd_t a)
+      (lc : LV.lin_cond env t csm prd)
+      (sl0 : sl_f (lc_pre lc)) (sl_ro : sl_f (lc_ro lc))
+  : Type0
+  = LV.tree_req lc (append_vars_mask csm sl0 sl_ro)
+
+let lc_ens
+      (#a : Type u#a) (#env : vprop_list) (#t : M.prog_tree a) (#csm : LV.csm_t env) (#prd : LV.prd_t a)
+      (lc : LV.lin_cond env t csm prd)
+      (sl0 : sl_f (lc_pre lc)) (x : a) (sl1 : sl_f (lc_post lc x)) (sl_ro : sl_f (lc_ro lc))
+  : Type0
+  = LV.tree_ens lc (append_vars_mask csm sl0 sl_ro) x sl1
+
+let lc_spec_r
+      (#a : Type u#a) (#env : vprop_list) (#t : M.prog_tree a) (#csm : LV.csm_t env) (#prd : LV.prd_t a)
+      (lc : LV.lin_cond env t csm prd)
+  : M.spec_r a
+  = M.Mkspec_r (lc_pre lc) (lc_post lc) (lc_ro lc) (lc_req lc) (lc_ens lc)
+
+[@@ __LV2SF__]
+let lc_sf
+      (#a : Type u#a) (#env : vprop_list) (#t : M.prog_tree a) (#csm : LV.csm_t env) (#prd : LV.prd_t a)
+      (lc : LV.lin_cond env t csm prd)
+  : LV.gen_sf (lc_spec_r lc)
+  =
+    fun (sl0 : sl_f (lc_pre lc)) (sl_ro : sl_f (lc_ro lc)) ->
+      let sl0' = LV2SF.append_vars_mask_l csm (Fl.dlist_of_f sl0) (Fl.dlist_of_f sl_ro) in
+      (**) LV2SF.repr_SF_of_LV_sound lc sl0';
+      LV2SF.repr_SF_of_LV lc sl0'
+
+let rew_lc_sf_req
+      (#a : Type u#a) (#env : vprop_list) (#t : M.prog_tree a) (#csm : LV.csm_t env) (#prd : LV.prd_t a)
+      (lc : LV.lin_cond env t csm prd)
+      (sl0 : sl_f (lc_pre lc)) (sl_ro : sl_f (lc_ro lc))
+  : squash (lc_req lc sl0 sl_ro <==> SF.tree_req (lc_sf lc sl0 sl_ro))
+  = ()
+
+let rew_lc_sf_ens
+      (#a : Type u#a) (#env : vprop_list) (#t : M.prog_tree a) (#csm : LV.csm_t env) (#prd : LV.prd_t a)
+      (lc : LV.lin_cond env t csm prd)
+      (sl0 : sl_f (lc_pre lc)) (x : a) (sl1 : sl_f (lc_post lc x)) (sl_ro : sl_f (lc_ro lc))
+  : squash (lc_ens lc sl0 x sl1 sl_ro <==> SF.tree_ens (lc_sf lc sl0 sl_ro) x sl1)
+  = ()
+
+
+#push-options "--fuel 0 --ifuel 0 --z3rlimit 20"
+inline_for_extraction
+let lc_to_spc_steel_t__steel
+      (#a : Type u#a) (mr : M.repr SH.KSteel a)
+      (#env : vprop_list) (#csm : LV.csm_t env) (#prd : LV.prd_t a)
+      (lc : LV.lin_cond env mr.repr_tree csm prd {LV.lcsub_at_leaves lc})
+  : M.spc_steel_t SH.KSteel (lc_spec_r lc)
+  =
+    let tc = LV2M.repr_M_of_LV lc                              in
+    let sf = mr.repr_steel env (LV2M.res_env_f env csm prd) tc in
+    (**) LV2M.repr_M_of_LV_sound lc;
+    SH.steel_f (fun () ->
+      (**) let sl0    = gget_f (lc_pre lc)    in
+      (**) let sl_ro0 = gget_f (lc_ro  lc)    in
+      elim_filter_mask_append env csm;
+      (**) let sl0'   = gget_f env            in
+      let x = SH.steel_u sf () in
+      (**) let sl1'   = gget_f L.(lc_post lc x @ lc_ro lc) in
+      steel_elim_vprop_of_list_append_f (lc_post lc x) (lc_ro lc);
+      (**) let sl1    = gget_f (lc_post lc x) in
+      (**) let sl_ro1 = gget_f (lc_ro   lc)   in
+      (**) assert (Ghost.reveal sl1' == LV2M.res_env_app sl1 sl_ro1);
+      (**) assert (M.tree_ens _ tc sl0' x sl1');
+      (**) filter_append_vars_mask csm sl0 sl_ro0;
+      (**) assert (LV.tree_ens lc sl0' x sl1 /\ sl_ro0 == sl_ro1);
+      SA.return x
+    )
+
+inline_for_extraction
+let lc_to_spc_steel_t__atomic
+      (opened : Mem.inames) (#a : Type u#a) (mr : M.repr (SH.KAtomic opened) a)
+      (#env : vprop_list) (#csm : LV.csm_t env) (#prd : LV.prd_t a)
+      (lc : LV.lin_cond env mr.repr_tree csm prd {LV.lcsub_at_leaves lc})
+  : M.spc_steel_t (SH.KAtomic opened) (lc_spec_r lc)
+  =
+    let tc = LV2M.repr_M_of_LV lc                              in
+    let sf = mr.repr_steel env (LV2M.res_env_f env csm prd) tc in
+    (**) LV2M.repr_M_of_LV_sound lc;
+    SH.atomic_f #opened (fun () ->
+      (**) let sl0    = gget_f (lc_pre lc)    in
+      (**) let sl_ro0 = gget_f (lc_ro  lc)    in
+      elim_filter_mask_append env csm;
+      (**) let sl0'   = gget_f env            in
+      let x = SH.atomic_u sf () in
+      (**) let sl1'   = gget_f L.(lc_post lc x @ lc_ro lc) in
+      steel_elim_vprop_of_list_append_f (lc_post lc x) (lc_ro lc);
+      (**) let sl1    = gget_f (lc_post lc x) in
+      (**) let sl_ro1 = gget_f (lc_ro   lc)   in
+      (**) assert (Ghost.reveal sl1' == LV2M.res_env_app sl1 sl_ro1);
+      (**) assert (M.tree_ens _ tc sl0' x sl1');
+      (**) filter_append_vars_mask csm sl0 sl_ro0;
+      (**) assert (LV.tree_ens lc sl0' x sl1 /\ sl_ro0 == sl_ro1);
+      SA.return x
+    )
+
+inline_for_extraction
+let lc_to_spc_steel_t__ghost
+      (opened : Mem.inames) (#a : Type u#a) (mr : M.repr (SH.KGhost opened) a)
+      (#env : vprop_list) (#csm : LV.csm_t env) (#prd : LV.prd_t a)
+      (lc : LV.lin_cond env mr.repr_tree csm prd {LV.lcsub_at_leaves lc})
+  : M.spc_steel_t (SH.KGhost opened) (lc_spec_r lc)
+  =
+    let tc = LV2M.repr_M_of_LV lc                              in
+    let sf = mr.repr_steel env (LV2M.res_env_f env csm prd) tc in
+    (**) LV2M.repr_M_of_LV_sound lc;
+    SH.ghost_f #opened (fun () ->
+      (**) let sl0    = gget_f (lc_pre lc)    in
+      (**) let sl_ro0 = gget_f (lc_ro  lc)    in
+      elim_filter_mask_append env csm;
+      (**) let sl0'   = gget_f env            in
+      let x = SH.ghost_u sf () in
+      (**) let sl1'   = gget_f L.(lc_post lc x @ lc_ro lc) in
+      steel_elim_vprop_of_list_append_f (lc_post lc x) (lc_ro lc);
+      (**) let sl1    = gget_f (lc_post lc x) in
+      (**) let sl_ro1 = gget_f (lc_ro   lc)   in
+      (**) assert (Ghost.reveal sl1' == LV2M.res_env_app sl1 sl_ro1);
+      (**) assert (M.tree_ens _ tc sl0' x sl1');
+      (**) filter_append_vars_mask csm sl0 sl_ro0;
+      (**) assert (LV.tree_ens lc sl0' x sl1 /\ sl_ro0 == sl_ro1);
+      (**) noop ();
+      x
+    )
+#pop-options
+
+inline_for_extraction
+let lc_to_spc_steel_t
+      (#ek : SH.effect_kind) (#a : Type u#a) (mr : M.repr ek a)
+      (#env : vprop_list) (#csm : LV.csm_t env) (#prd : LV.prd_t a)
+      (lc : LV.lin_cond env mr.repr_tree csm prd {LV.lcsub_at_leaves lc})
+  : M.spc_steel_t ek (lc_spec_r lc)
+  =
+    match ek with
+    | SH.KSteel    -> lc_to_spc_steel_t__steel    mr lc
+    | SH.KAtomic o -> lc_to_spc_steel_t__atomic o mr lc
+    | SH.KGhost  o -> lc_to_spc_steel_t__ghost  o mr lc
+
+
+(*** [lin_cond_st] *)
+
+/// [lin_cond_st env t must_csm must_prd csm1 prd1] ("lin_cond such that") is used to build a [lin_cond] consuming at
+/// least [must_csm] and producing at least [must_prd]. It allows other variables to be consumed ([csm1]) or
+/// produced ([prd1]).
+
+#push-options "--ifuel 0 --fuel 0"
+
+type lin_cond_st
+       (env : vprop_list) (#a : Type u#a) (t : M.prog_tree a)
+       (must_csm : LV.csm_t env) (must_prd : LV.prd_t a)
+       (csm1 : LV.csm_t Msk.(filter_mask (mask_not must_csm) env)) (prd1 : LV.prd_t a)
+  = lc : LV.lin_cond env #a t (Msk.mask_comp_or must_csm csm1) L.(fun x -> must_prd x @ prd1 x)
+       { LV.lcsub_at_leaves lc }
+
+let pequiv_append_02 (#a : Type) (l0 l1 l2 l3 : list a)
+  : Perm.pequiv L.(l0 @ l1 @ l2 @ l3) L.(l0 @ l2 @ l1 @ l3)
+  =
+    L.append_assoc l1 l2 l3; L.append_assoc l2 l1 l3;
+    U.cast _
+    Perm.(pequiv_append (pequiv_refl l0)
+         (pequiv_append (pequiv_append_swap l1 l2)
+                        (pequiv_refl l3)))
+
+[@@ __cond_solver__]
+let build_lin_cond_st_prd_f
+      (prd0 env must_prd : vprop_list) (must_csm : LV.csm_t env)
+      (post_f : LV.eq_injection_l must_prd L.(prd0 @ env))
+  : (let n0 = L.length prd0          in
+     let n1 = L.length env           in
+     let m0 = LV.eij_trg_mask post_f in
+     (**) L.splitAt_length n0 m0;
+     let m0a, m0b = L.splitAt n0 m0  in
+     let m0a : Ll.vec n0 bool = m0a  in
+     let m0b : Ll.vec n1 bool = m0b  in
+     Perm.pequiv_list
+      L.(prd0 @ Msk.(filter_mask (mask_or m0b must_csm) env))
+      L.(must_prd @ Msk.(filter_mask (mask_not m0a) prd0) @ filter_diff m0b must_csm env))
+  = Msk.(
+    let n0 = L.length prd0          in
+    let n1 = L.length env           in
+    let m0 = LV.eij_trg_mask post_f in
+    (**) L.splitAt_length n0 m0;
+    let m0a, m0b = L.splitAt n0 m0  in
+    let m0a : Ll.vec n0 bool = m0a  in
+    let m0b : Ll.vec n1 bool = m0b  in
+
+    let must_csm' = mask_diff m0b must_csm in
+
+    let flt00 = filter_mask m0a prd0                                   in
+    let flt01 = filter_mask (mask_not m0a) prd0                        in
+    let flt10 = filter_mask m0b env                                    in
+    let flt11 = filter_mask must_csm' (filter_mask (mask_not m0b) env) in
+
+    Ll.list_extensionality (mask_or m0b must_csm) (mask_comp_or m0b must_csm') (fun i -> ());
+    assert (filter_diff m0b must_csm env == flt11);
+    U.assert_by L.(filter_mask m0 (prd0 @ env) == flt00 @ flt10) (fun () ->
+      Ll.lemma_splitAt_append n0 m0;
+      filter_mask_append m0a m0b prd0 env);
+
+    let f0 : Perm.pequiv L.(flt00 @ flt10) must_prd
+      = U.cast _ (LV.eij_equiv post_f)           in
+    let f1 : Perm.pequiv prd0 L.(flt00 @ flt01)
+      = mask_pequiv_append m0a prd0              in
+    let f2 : Perm.pequiv (filter_mask (mask_comp_or m0b must_csm') env) L.(flt10 @ flt11)
+      = mask_or_pequiv_append m0b must_csm' env  in
+
+    L.append_assoc flt00 flt01 L.(flt10 @ flt11);
+    let f3 : Perm.pequiv L.(prd0 @ filter_mask (mask_comp_or m0b must_csm') env)
+                         L.(flt00 @ flt01 @ flt10 @ flt11)
+      = Perm.pequiv_append f1 f2                 in
+    L.append_assoc flt00 flt10 L.(flt01 @ flt11);
+    let f4 : Perm.pequiv L.(flt00 @ flt01 @ flt10 @ flt11)
+                         L.((flt00 @ flt10) @ (flt01 @ flt11))
+      = pequiv_append_02 flt00 flt01 flt10 flt11 in
+
+    let f : Perm.pequiv L.(prd0 @ filter_mask (mask_comp_or m0b must_csm') env)
+                        L.(must_prd @ (flt01 @ flt11))
+      = Perm.(pequiv_trans f3
+             (pequiv_trans f4
+             (pequiv_append f0 (pequiv_refl L.(flt01 @ flt11)))))
+    in Perm.perm_f_to_list f)
+
+[@@ __cond_solver__]
+let __build_lin_cond_st
+      (env : vprop_list) (#a : Type u#a) (t : M.prog_tree a)
+      (csm0 : LV.csm_t env) (prd0 : LV.prd_t a)
+      (ct : LV.lin_cond env t csm0 prd0)
+      (must_csm : LV.csm_t env) (must_prd : LV.prd_t a)
+      (post_f : (x : a) -> LV.eq_injection_l (must_prd x) (LV.res_env env csm0 (prd0 x)))
+      (csm' : Msk.(mask_t (filter_mask (mask_not csm0) env)))
+      (csm'_eq : (x : a) -> squash (
+        let n0 = L.length (prd0 x)          in
+        let m0 = LV.eij_trg_mask (post_f x) in
+        (**) L.splitAt_length n0 m0;
+        csm' = (L.splitAt n0 m0)._2))
+  : lin_cond_st env t must_csm must_prd
+        Msk.(mask_diff must_csm (mask_comp_or csm0 csm'))
+        (fun x ->
+          let n0 = L.length (prd0 x)          in
+          let m0 = LV.eij_trg_mask (post_f x) in
+          (**) L.splitAt_length n0 m0;
+          let m0a : Ll.vec n0 bool = (L.splitAt n0 m0)._1 in
+          L.(Msk.filter_mask (Msk.mask_not m0a) (prd0 x)
+           @ filter_diff (Msk.mask_comp_or csm0 csm') must_csm env))
+  =
+    let csm1 : Msk.(mask_t (filter_mask (mask_not csm0) env))
+             = Msk.(mask_or csm' (mask_diff csm0 must_csm))     in
+    let prd1 x =
+      let n0 = L.length (prd0 x)                                in
+      let m0 = LV.eij_trg_mask (post_f x)                       in
+      (**) L.splitAt_length n0 m0;
+      let m0a : Ll.vec n0 bool = (L.splitAt n0 m0)._1           in
+      L.(Msk.filter_mask (Msk.mask_not m0a) (prd0 x)
+       @ filter_diff (Msk.mask_comp_or csm0 csm') must_csm env) in
+    Msk.(calc (==) {
+      LV.bind_csm env csm0 csm1 <: list bool;
+    == { Ll.list_extensionality_sq (fun i -> ()) }
+      mask_or must_csm (mask_comp_or csm0 csm');
+    == { mask_comp_or_mask_diff must_csm (mask_comp_or csm0 csm') }
+      mask_comp_or must_csm (mask_diff must_csm (mask_comp_or csm0 csm'));
+    });
+    let prd_f (x : a) : Perm.pequiv_list (LV.sub_prd env csm0 (prd0 x) csm1) L.(must_prd x @ prd1 x)
+      =
+        let n0 = L.length (prd0 x)              in
+        let n1 = Msk.(mask_len (mask_not csm0)) in
+        let m0 = LV.eij_trg_mask (post_f x)     in
+        (**) L.splitAt_length n0 m0;
+        let m0a, m0b = L.splitAt n0 m0          in
+        let m0a : Ll.vec n0 bool = m0a          in
+        let m0b : Ll.vec n1 bool = m0b          in
+        U.assert_by (csm' == m0b) (fun () -> csm'_eq x);
+        let env1      = Msk.(filter_mask (mask_not csm0) env) in
+        let must_csm1 = Msk.(mask_diff csm0 must_csm)         in
+        assert (LV.sub_prd env csm0 (prd0 x) csm1
+          == L.(prd0 x @ Msk.(filter_mask (mask_or m0b must_csm1) env1)));
+        Msk.(calc (==) {
+          filter_diff m0b (mask_diff csm0 must_csm) (filter_mask (mask_not csm0) env);
+        == { }
+          filter_mask (mask_diff m0b (mask_diff csm0 must_csm))
+            (filter_mask (mask_not m0b) (filter_mask (mask_not csm0) env));
+        == { filter_mask_and (mask_not csm0) (mask_not m0b) must_csm;
+             filter_mask_and (mask_not csm0) (mask_not m0b) env }
+          filter_mask (filter_mask (mask_comp_and (mask_not csm0) (mask_not m0b)) must_csm)
+            (filter_mask (mask_comp_and (mask_not csm0) (mask_not m0b)) env);
+        == { mask_not_comp_or csm0 m0b }
+          filter_mask (filter_mask (mask_not (mask_comp_or csm0 m0b)) must_csm)
+            (filter_mask (mask_not (mask_comp_or csm0 m0b)) env);
+        == { }
+          filter_diff (mask_comp_or csm0 m0b) must_csm env;
+        });
+        assert L.(must_prd x @ prd1 x
+               == must_prd x @ Msk.(filter_mask (mask_not m0a) (prd0 x)) @ filter_diff m0b must_csm1 env1);
+        build_lin_cond_st_prd_f (prd0 x) env1 (must_prd x) must_csm1 (post_f x)
+    in
+    let ct' = LV.LCsub env csm0 prd0 ct csm1 L.(fun x -> must_prd x @ prd1 x) prd_f in
+    (**) LV.lc_sub_push_at_leaves env ct';
+    LV.lc_sub_push ct'
+
+
+noeq
+type test_lin_cond_st env #a t must_csm must_prd =
+  | TestLinCondSt : (csm1 : _) -> (prd1 : _) ->
+                    lin_cond_st env #a t must_csm must_prd csm1 prd1 ->
+                    test_lin_cond_st env t must_csm must_prd
+
+#push-options "--fuel 5"
+let test_lin_cond_st_0 (v : int -> vprop')
+  : test_lin_cond_st [v 0; v 1; v 2; v 3]
+      M.(Tspec unit (M.spec_r_exact (Mkspec_r [v 0] (fun _ -> [v 4; v 5]) [v 1] (fun _ _ -> True) (fun _ _ _ _ -> True))))
+      [true; false; true; false] (fun _ -> [v 4; v 1])
+  = _ by (
+    apply (`TestLinCondSt);
+    apply_raw (`__build_lin_cond_st);
+    // ct
+    dismiss (); dismiss ();
+    build_lin_cond default_flags None;
+    // post_f
+    let x = intro () in
+    norm_lc ();
+    build_eq_injection_l default_flags dummy_ctx;
+    // csm'_eq
+    dismiss ();
+    let x = intro () in
+    norm_lc ();
+    trefl ()
+  )
+#pop-options
+
+[@@ __cond_solver__]
+let __normalize_lin_cond_st
+       (env : vprop_list) (#a : Type u#a) (t : M.prog_tree a)
+       (must_csm : LV.csm_t env) (must_prd : LV.prd_t a)
+       (csm1 : LV.csm_t Msk.(filter_mask (mask_not must_csm) env)) (prd1 : LV.prd_t a)
+       (lc : lin_cond_st env t must_csm must_prd csm1 prd1)
+       (lc1 : lin_cond_st env t must_csm must_prd csm1 prd1)
+       (_ : squash (lc1 == lc))
+       (csm2 : LV.csm_t Msk.(filter_mask (mask_not must_csm) env)) (prd2 : LV.prd_t a)
+       (_ : squash (csm2 == csm1 /\ prd2 == prd1))
+  : lin_cond_st env t must_csm must_prd csm2 prd2
+  = lc1
+
+#pop-options
+
+#push-options "--ifuel 1"
+/// Solves a goal [lin_cond_st env t must_csm must_prd ?csm1 ?prd1]
+let build_lin_cond_st (fr : flags_record) (ctx : cs_context) : Tac unit
+  =
+    apply_raw (`__normalize_lin_cond_st);
+    // lc
+      dismiss (); dismiss ();
+      apply_raw (`__build_lin_cond_st);
+      // ct
+      dismiss (); dismiss ();
+      build_lin_cond fr None;
+      // post_f
+      let x = intro () in
+      norm_lc ();
+      build_eq_injection_l fr ctx;
+      // csm'_eq
+      dismiss ();
+      let x = intro () in
+      norm_lc ();
+      cs_try trefl fr ctx (fun m -> fail (m (Fail_dependency "csm" x) []));
+    // lc1 <-
+    dismiss ();
+    norm [
+      delta_only (L.append __delta_list [
+        `%L.splitAt; `%L.mem; `%Mktuple2?._1; `%Mktuple2?._2; `%L.map2;
+        `%Perm.perm_f_to_list; `%Perm.comp; `%Perm.perm_f_append; `%Perm.mk_perm_f; `%Perm.perm_f_of_pair;
+        `%Perm.pequiv_append_swap; `%pequiv_append_02;
+        `%LV.eij_equiv; `%LV.eij_equiv_f]);
+      delta_attr [`%__cond_solver__; `%Learn.Tactics.Util.__tac_helper__; `%Msk.__mask__; `%LV.__lin_cond__];
+      delta_qualifier ["unfold"];
+      iota; zeta; primops];
+    trefl ();
+    // csm2, prd2 <-
+    norm_lc ();
+    split (); trefl (); trefl ()
+#pop-options
