experiment/Experiment.Steel.Test.Extract.fst
@@ -34,3 +34,17 @@ let test_ghost (r : ref U32.t)
   : Steel U32.t (vptr r) (fun _ -> vptr r)
       (requires fun _ -> True) (ensures fun h0 _ h1 -> frame_equalities (vptr r) h0 h1)
   = Test.test_ghost r ()
+
+
+let test_slrewrite (r0 r1 r2 : ref U32.t)
+  : Steel unit
+      (vptr r0 `star` vptr r1) (fun _ -> vptr r2 `star` vptr r1)
+      (requires fun _ -> r0 == r2)
+      (ensures  fun h0 _ h1 -> sel r0 h0 == sel r2 h1 /\ sel r1 h0 == sel r1 h1)
+  = Test.test_slrewrite r0 r1 r2 ()
+
+let test_with_invariant_g (r0 : ghost_ref U32.t) (r1 : ref U32.t) (i : inv (ghost_vptr r0))
+  : Steel (Ghost.erased U32.t)
+      (vptr r1) (fun _ -> vptr r1)
+      (requires fun _ -> True) (ensures fun h0 _ h1 -> frame_equalities (vptr r1) h0 h1)
+  = Test.test_with_invariant_g r0 r1 i ()
